# 题目

（1） $$(\frac{4}{5}+( \frac{3}{8}-\frac{1}{4}))$$

（2） $$(2-\frac{3}{7}-\frac{4}{7})$$

（3） $$(\frac{5}{8}-\frac{1}{3}+\frac{5}{12})$$
    
# 解题思路

（1）对于 $$(\frac{4}{5}+( \frac{3}{8}-\frac{1}{4}))$$，先计算括号内的式子， $$(\frac{3}{8}-\frac{1}{4}=\frac{3}{8}-\frac{2}{8}=\frac{1}{8})$$，然后再计算 $$(\frac{4}{5}+\frac{1}{8})$$，通分得到 $$(\frac{32}{40}+\frac{5}{40}=\frac{37}{40})$$。

（2）对于 $$(2-\frac{3}{7}-\frac{4}{7})$$，观察发现后两项分母相同，可以利用减法的性质先将后两项相加， $$(\frac{3}{7}+\frac{4}{7} = 1)$$，然后 $$(2 - 1=1)$$。

（3）对于 $$(\frac{5}{8}-\frac{1}{3}+\frac{5}{12})$$，先通分， $$(\frac{5}{8}=\frac{15}{24})$$， $$(\frac{1}{3}=\frac{8}{24})$$， $$(\frac{5}{12}=\frac{10}{24})$$，则原式变为 $$(\frac{15}{24}-\frac{8}{24}+\frac{10}{24}=\frac{15 - 8+10}{24}=\frac{17}{24})$$。
    
# 答案

（1） $$(\frac{37}{40})$$
（2） $$(1)$$
（3） $$(\frac{17}{24})$$
